theories/rust_typing/existentials.v
@@ -550,7 +550,7 @@ Section stratify.
     iExists L2. iFrame. iPoseProof ("HT" with "HR2") as "$". iModIntro.
     iSplitR; last iSplitR.
     - simpl. iPureIntro.
-      intros ly1 ly2 Hly1 HLy2. f_equiv. by eapply syn_type_has_layout_inj.
+      apply syn_type_size_eq_refl.
     - simpl. eauto.
     - iIntros (v) "Hv0".
       iEval (rewrite /ty_own_val/=).
